ECCA_typing.v
@@ -1,5 +1,5 @@
 Require Export ECCA_equiv.
-
+Require Export ECCA_core_lemmas.
 (*
 ================================
 =======--Type System--==========
@@ -69,23 +69,21 @@ Inductive ECCA_has_type: ECCAenv -> ECCAexp -> ECCAexp -> Prop :=
 | aT_Lam (g: ECCAenv) (x: name) (A e B: ECCAexp) :
   (ECCA_has_type (g & x ~ Assum A) (open x e) (open x B)) ->
   (g |- (eAbs A e) : (ePi A B))
-(* ECCA_has_type: ECCAenv -> ECCAconf -> ECCAconf -> Prop := *)
 | aT_Let (g: ECCAenv) (n m A B: ECCAexp) (x: name):
   (g |- n : A) ->
   (ECCA_has_type (g & x ~ Def n A) (open x m) (open x B)) ->
   (g |- (eLet n m) : (bind n B))
-(* | aT_If (g: ECCAenv) (B U e1 e2: ECCAexp) (e: ECCAexp) (x: atom):
-  ECCA_has_type (Assum g x eBool) B U -> 
-  g |- e : eBool ->
-  ECCA_has_type (Eq g e eTru) e1 (subst x eTru B) ->
-  ECCA_has_type (Eq g e eFls) e2 (subst x eFls B) -> 
-  g |- (eIf e e1 e2) : (subst x e B) *)
+| aT_If (g: ECCAenv) (B U e1 e2: ECCAexp) (e: ECCAexp) (x y: name):
+  ECCA_has_type (g & x ~ Assum eBool) (open x B) U -> 
+  ECCA_has_type g e eBool ->
+  ECCA_has_type (g & y ~ Eq e eTru) e1 (bind eTru B) ->
+  ECCA_has_type (g & y ~ Eq e eFls) e2 (bind eFls B) -> 
+  (g |- (eIf e e1 e2) : (bind e B)) 
 | aT_Conv (g: ECCAenv) (e A B U: ECCAexp) :
   (g |- e : A) ->
   (g |- B : U) ->
   (ECCA_sub_type g A B) ->
   (g |- e : B)
-(* ECCA_has_type: ECCAenv -> ECCAcomp -> ECCAconf -> Prop := *)
 | aT_App (g: ECCAenv) (x: name) (e e': ECCAexp) (A' B: ECCAexp) :
   (g |- e : (ePi A' B)) ->
   (g |- e' : A') ->
@@ -96,18 +94,11 @@ Inductive ECCA_has_type: ECCAenv -> ECCAexp -> ECCAexp -> Prop :=
 | aT_Snd (g: ECCAenv) (e: ECCAexp) (A B: ECCAexp) :
   (g |- e: (eSig A B)) ->
   (g |- (eSnd e): (bind (eFst e) B)) 
-(* | aT_Subst (x: atom) (g: ECCAenv) (A B U: ECCAexp) (e e1 e2: ECCAexp):
-  (ECCA_has_type (Assum g x A) B U) ->
-  g |- e1: A -> 
-  g |- e2: A ->
-  g |- e: (subst x e1 B) ->
-  ECCA_LookupEqR g e1 e2 ->
-  g |- (eSubst e1 e2 e): (subst x e2 B)  *)
 where "g '|-' a ':' b" := (ECCA_has_type g a b) : ECCA_scope
 with 
 (* ECCA Well-Formed Environments *)
 ECCA_Env_WF: ECCAenv -> Prop :=
-| W_Empty (g: ECCAenv) :
+| W_Empty (g: @ECCAenv 0) :
   ECCA_Env_WF ctx_empty
 | W_Assum (g: ECCAenv) (x: name) (A U: ECCAexp) :
   ECCA_Env_WF g ->
@@ -120,5 +111,168 @@ ECCA_Env_WF: ECCAenv -> Prop :=
   ECCA_Env_WF (g & x ~ Def e A)
 (* | W_Eq  *)
 .
+
+(* 
+=====================================
+Well boundedness wrt Type Environments 
+=====================================
+*)
+
+Inductive ECCA_wf {V: nat}: ECCAenv -> ECCAexp -> Prop :=
+| wf_Prop (g: ECCAenv) :
+    ECCA_Env_WF g ->
+    ECCA_wf g (eUni uProp)
+| wf_Type (g: ECCAenv) (i: nat) :
+    ECCA_Env_WF g ->
+    ECCA_wf g (eUni (uType i))
+| wf_Var (g: ECCAenv) (x: atom) (A: ECCAexp) :
+    (assumes g x A) -> (* this needs adjustment *)
+    ECCA_wf g (eId x)
+| wf_Bool (g: ECCAenv) :
+    ECCA_Env_WF g ->
+    ECCA_wf g eBool
+| wf_True (g: ECCAenv):
+    ECCA_Env_WF g ->
+    ECCA_wf g eTru
+| wf_False (g: ECCAenv):
+    ECCA_Env_WF g ->
+    ECCA_wf g eFls
+| wf_Sig (g: ECCAenv) (x: name) (A B: ECCAexp) (i: nat) :
+    ECCA_wf g A ->
+    ECCA_wf (g & x ~ Assum A) (open x B) ->
+    ECCA_wf g (eSig A B)
+| wf_Pair (g: ECCAenv) (v1 v2: ECCAexp) (A B: ECCAexp) (x: name) :
+    ECCA_wf g v1 ->
+    ECCA_wf g v2 ->
+    ECCA_wf g A ->
+    ECCA_wf (g & x ~ Def v1 A) (open x B) ->
+    ECCA_wf g (ePair v1 v2 (eSig A B))
+| wf_Pi (g: ECCAenv) (x: name) (A B: ECCAexp) :
+    ECCA_wf g A ->
+    ECCA_wf (g & x ~ Assum A) (open x B) ->
+    ECCA_wf g (ePi A B)
+| wf_Lam (g: ECCAenv) (x: name) (A e B: ECCAexp) :
+    ECCA_wf (g & x ~ Assum A) (open x B) ->
+    ECCA_wf (g & x ~ Assum A) (open x e) ->
+    ECCA_wf g (eAbs A e)
+| wf_Let (g: ECCAenv) (n m A B: ECCAexp) (x: name):
+    ECCA_wf g n ->
+    ECCA_wf g A ->
+    ECCA_wf (g & x ~ Def n A) (open x B) ->
+    ECCA_wf (g & x ~ Def n A) (open x m) ->
+    ECCA_wf g (eLet n m)
+| wf_If (g: ECCAenv) (B e1 e2: ECCAexp) (e: ECCAexp) (x y: name):
+    ECCA_wf (g & x ~ Assum eBool) (open x B) -> 
+    ECCA_wf g e ->
+    ECCA_wf (g & y ~ Eq e eTru) e1 ->
+    ECCA_wf (g & y ~ Eq e eFls) e2 -> 
+    ECCA_wf g (eIf e e1 e2)
+| wf_App (g: ECCAenv) (x: name) (e e': ECCAexp):
+    ECCA_wf g e ->
+    ECCA_wf g e' ->
+    ECCA_wf g (eApp e e')
+| wf_Fst (g: ECCAenv) (e: ECCAexp) :
+    ECCA_wf g e ->
+    ECCA_wf g (eFst e)
+| wf_Snd (g: ECCAenv) (e: ECCAexp) :
+    ECCA_wf g e ->
+    ECCA_wf g (eSnd e)
+.
+
+(*
+Inductive ECCAval {V: nat}: Type :=
+  | Id (x: @atom V)
+  | Uni (U: ECCuni)
+  | Pi (A: ECCAconf) (B: @ECCAconf (S V))
+  | Abs (A: ECCAconf) (B: @ECCAconf (S V))
+  | Sig (A: ECCAconf) (B: @ECCAconf (S V))
+  | Pair (v1 v2: ECCAval) (A: @ECCAconf V)
+  | Tru
+  | Fls
+  | Bool
+with
+ECCAconf {V: nat}: Type :=
+  | Comp (e: ECCAcomp)
+  | Let (A: ECCAcomp) (B: @ECCAconf (S V))
+  | If (v: ECCAval) (m1 m2: ECCAconf)
+with
+ECCAcomp {V: nat}: Type :=
+  | App (v1 v2: ECCAval)
+  | Val (v: ECCAval)
+  | Fst (v: ECCAval)
+  | Snd (v: ECCAval)
+.*)
+
+Check open.
+Parameter open_conf: name -> @ECCAconf 1 -> @ECCAconf 0.
+
+Inductive ECCA_val_wf {V: nat}: @ECCAenv 0 -> ECCAval -> Prop :=
+| wf_val_Id (g: ECCAenv) (A: ECCAexp) (x: atom):
+    (assumes g x A) -> (* this needs adjustment *)
+    ECCA_val_wf g (Id x)
+| wf_val_Prop (g: ECCAenv) :
+    ECCA_Env_WF g ->
+    ECCA_val_wf g (Uni uProp)
+| wf_val_Type (g: ECCAenv) (i: nat) :
+    ECCA_Env_WF g ->
+    ECCA_val_wf g (Uni (uType i))
+| wf_val_Bool (g: ECCAenv) :
+    ECCA_Env_WF g ->
+    ECCA_val_wf g Bool
+| wf_val_True (g: ECCAenv):
+    ECCA_Env_WF g ->
+    ECCA_val_wf g Tru
+| wf_val_False (g: ECCAenv):
+    ECCA_Env_WF g ->
+    ECCA_val_wf g Fls
+| wf_val_Sig (g: ECCAenv) (x: name) (A B: ECCAconf) (i: nat) :
+    ECCA_conf_wf g A ->
+    ECCA_conf_wf (g & x ~ Assum (flattenECCAconf A)) (open_conf x B) ->
+    ECCA_val_wf g (Sig A B)
+| wf_val_Pair (g: ECCAenv) (v1 v2: ECCAval) (A B: ECCAconf) (x: name) :
+    ECCA_val_wf g v1 ->
+    ECCA_val_wf g v2 ->
+    ECCA_conf_wf g A ->
+    ECCA_conf_wf (g & x ~ Def (flattenECCAval v1) (flattenECCAconf A)) (open_conf x B) ->
+    ECCA_val_wf g (Pair v1 v2 (Sig A B))
+| wf_val_Pi (g: ECCAenv) (x: name) (A B: ECCAconf) :
+    ECCA_conf_wf g A ->
+    ECCA_conf_wf (g & x ~ Assum (flattenECCAconf A)) (open_conf x B) ->
+    ECCA_val_wf g (Pi A B)
+| wf_val_Lam (g: ECCAenv) (x: name) (A e: ECCAconf) :
+    ECCA_conf_wf (g & x ~ Assum (flattenECCAconf A)) (open_conf x e) ->
+    ECCA_val_wf g (Abs A e)
+with ECCA_conf_wf {V: nat}: ECCAenv -> ECCAconf -> Prop :=  
+| wf_conf_Comp (g: ECCAenv) (e: ECCAcomp):
+    ECCA_comp_wf g e ->
+    ECCA_conf_wf g (Comp e)
+| wf_conf_Let (g: ECCAenv) (n: ECCAcomp) (m A: ECCAconf) (x: name):
+    ECCA_comp_wf g n ->
+    ECCA_conf_wf g A ->
+    ECCA_conf_wf (g & x ~ Def (flattenECCAcomp n) (flattenECCAconf A)) (open_conf x m) ->
+    ECCA_conf_wf g (Let n m)
+| wf_conf_If (g: ECCAenv) (v: ECCAval) (B m1 m2: ECCAconf) (x y: name):
+    ECCA_conf_wf (g & x ~ Assum eBool) (open_conf x B) -> 
+    ECCA_val_wf g v ->
+    ECCA_conf_wf (g & y ~ Eq (flattenECCAval v) eTru) m1 ->
+    ECCA_conf_wf (g & y ~ Eq (flattenECCAval v) eFls) m2 -> 
+    ECCA_conf_wf g (If v m1 m2)
+with ECCA_comp_wf {V: nat}: ECCAenv -> ECCAcomp -> Prop :=
+| wf_comp_Val (g: ECCAenv) (v: ECCAval):
+    ECCA_val_wf g v ->
+    ECCA_comp_wf g (Val v)
+| wf_comp App (g: ECCAenv) (x: name) (v v': ECCAval):
+    ECCA_val_wf g v ->
+    ECCA_val_wf g v' ->
+    ECCA_comp_wf g (App v v')
+| wf_comp_Fst (g: ECCAenv) (v: ECCAval) :
+    ECCA_val_wf g v ->
+    ECCA_comp_wf g (Fst v)
+| wf_comp_Snd (g: ECCAenv) (v: ECCAval) :
+    ECCA_val_wf g v ->
+    ECCA_comp_wf g (Snd v)
+.
+
 Hint Constructors ECCA_has_type.
 Hint Constructors ECCA_Env_WF.
+
